code generation

theories/Compositional_Structures/Basic_Modules/Component_Types/Electoral_Module_Ref.thy
@@ -8,29 +8,21 @@ begin
 
 type_synonym 'a Electoral_Module_Ref = "'a set \<Rightarrow> 'a Profile_List \<Rightarrow> 'a Result nres"
 
+type_synonym 'a Electoral_Module_Sep = "('a, unit) hashtable
+      \<Rightarrow> ('a array \<times> nat) list
+         \<Rightarrow> (('a, unit) hashtable \<times> ('a, unit) hashtable \<times> ('a, unit) hashtable) Heap"
+
+
 abbreviation elec_mod_rel_orig :: "('a \<times> 'a) set \<Rightarrow> 
   ('a Electoral_Module \<times> 'a Electoral_Module) set" where
   "elec_mod_rel_orig R \<equiv> \<langle>\<langle>R\<rangle>set_rel , \<langle>\<langle>\<langle>R \<times>\<^sub>r R\<rangle>set_rel\<rangle>list_rel , 
   \<langle>R\<rangle>set_rel \<times>\<^sub>r \<langle>R\<rangle>set_rel \<times>\<^sub>r \<langle>R\<rangle>set_rel\<rangle>fun_rel\<rangle>fun_rel" 
 
-abbreviation elec_mod_rel_orig_nres :: "('a \<times> 'a) set \<Rightarrow> 
-  (('a set \<Rightarrow> 'a Profile \<Rightarrow> 'a Result nres) \<times> ('a::{default, heap, hashable} set \<Rightarrow> 'a Profile \<Rightarrow> 'a Result nres)) set" where
-  "elec_mod_rel_orig_nres R \<equiv> \<langle>\<langle>R\<rangle>set_rel , \<langle>\<langle>\<langle>R \<times>\<^sub>r R\<rangle>set_rel\<rangle>list_rel , 
-  \<langle>\<langle>R\<rangle>set_rel \<times>\<^sub>r \<langle>R\<rangle>set_rel \<times>\<^sub>r \<langle>R\<rangle>set_rel\<rangle>nres_rel\<rangle>fun_rel\<rangle>fun_rel" 
-
-abbreviation elec_mod_rel_ref :: "('a \<times> 'a) set \<Rightarrow> 
-  (('a set \<Rightarrow> 'a Profile_List \<Rightarrow> 'a Result) \<times> ('a set \<Rightarrow> 'a Profile_List \<Rightarrow> 'a Result)) set" where
-  "elec_mod_rel_ref R \<equiv> \<langle>\<langle>R\<rangle>set_rel , \<langle>\<langle>\<langle>R\<rangle>list_rel\<rangle>list_rel , 
-  \<langle>R\<rangle>set_rel \<times>\<^sub>r \<langle>R\<rangle>set_rel \<times>\<^sub>r \<langle>R\<rangle>set_rel\<rangle>fun_rel\<rangle>fun_rel" 
-
-abbreviation elec_mod_data_rel :: "('a \<times> 'a) set \<Rightarrow> 
-('a Electoral_Module_Ref \<times> ('a set \<Rightarrow> 'a Profile \<Rightarrow> 'a Result nres)) set" where
-  "elec_mod_data_rel R \<equiv> \<langle>R\<rangle>set_rel \<rightarrow> profile_rel 
-  \<rightarrow> \<langle>\<langle>R\<rangle>set_rel \<times>\<^sub>r \<langle>R\<rangle>set_rel \<times>\<^sub>r \<langle>R\<rangle>set_rel\<rangle>nres_rel"
-
-abbreviation elec_mod_nresc_rel :: "('a \<times> 'a) set \<Rightarrow> 
-('a Electoral_Module_Ref \<times> ('a set \<Rightarrow> 'a Profile \<Rightarrow> 'a Result)) set" where
-  "elec_mod_nresc_rel R \<equiv> {(emref, em). (emref, RETURN oo em) \<in> elec_mod_data_rel R}"
+abbreviation elec_mod_sep_rel where 
+  "elec_mod_sep_rel R \<equiv> [\<lambda>(a, b).
+           finite_profile a b]\<^sub>a (alts_set_impl_assn R)\<^sup>k *\<^sub>a 
+    (list_assn (hr_comp (ballot_impl_assn R) ballot_rel))\<^sup>k 
+        \<rightarrow> (result_impl_assn R)"
 
 
 end
