theories/Compositional_Structures/Sepref_Bindings.thy
@@ -26,10 +26,20 @@ lemma condorcet_aux:
   done
 
 
-sepref_decl_op  (no_def) borda ::  "elec_mod_rel_orig R" where "R = Id"
+sepref_decl_op  (no_def) "borda :: 'a::{default, heap, hashable} Electoral_Module" 
+  ::  "elec_mod_rel_orig R" where "R = Id"
     apply standard
   apply (rule nres_relI)
   apply simp done
+
+sepref_decl_op  (no_def) "elect_module :: 'a::{default, heap, hashable} Electoral_Module" 
+  ::  "elec_mod_rel_orig R" where "R = Id"
+  .
+
+(*sepref_decl_op  (no_def) condorcet ::  "elec_mod_rel_orig R" where "R = Id"
+    apply standard
+  apply (rule nres_relI)
+  apply simp done*)
 
 
 
@@ -37,24 +47,7 @@ sepref_decl_op  (no_def) borda ::  "elec_mod_rel_orig R" where "R = Id"
 sepref_decl_op (no_def) defer_equal_imp: "(defer_equal_condition)" :: 
   "\<langle>nat_rel, \<langle>(\<langle>R\<rangle>set_rel \<times>\<^sub>r \<langle>R\<rangle>set_rel \<times>\<^sub>r \<langle>R\<rangle>set_rel), \<langle>bool_rel\<rangle>nres_rel\<rangle>fun_rel\<rangle>fun_rel" 
   where "R = Id" .
-
-
-
-                              
-
-definition "alts_ref_assn \<equiv> hr_comp (alts_set_impl_assn id_assn) (\<langle>Id\<rangle>set_rel)"
-                                 
-
-definition "ballot_ref_assn \<equiv>  hr_comp (ballot_impl_assn id_assn) (\<langle>Id\<rangle>list_rel)"
-
-definition "alts_assn \<equiv> hr_comp alts_ref_assn (\<langle>Id\<rangle>set_rel)"
-                                           
-definition "result_set_one_step \<equiv> hr_comp (alts_set_impl_assn id_assn) (\<langle>Id\<rangle>set_rel)"
-
-definition "result_set_assn \<equiv> hr_comp(result_set_one_step) (\<langle>Id\<rangle>set_rel)"
-
-definition "ballot_assn \<equiv> hr_comp (hr_comp (ballot_impl_assn id_assn) ballot_rel) (\<langle>Id \<times>\<^sub>r Id\<rangle>set_rel)"
-
+                       
 
 locale refine_assns =
  notes  
@@ -66,10 +59,56 @@ locale refine_assns =
 begin
 
 
-sepref_decl_impl borda : borda_elim_sep.refine[FCOMP borda_ref_correct] 
-  by simp                                                              
 
 
+
+end
+
+locale sequence_sepref_direct = refine_assns +
+ fixes m :: "'a::{default, heap, hashable} Electoral_Module"  and
+  n :: "'a::{default, heap, hashable} Electoral_Module"
+  fixes m_sep :: "'a::{default, heap, hashable} Electoral_Module_Sep" 
+  and n_sep :: "'a::{default, heap, hashable} Electoral_Module_Sep" 
+  assumes module_m: "electoral_module m"
+  and module_n: "electoral_module n"
+  and m_sep_correct: "(uncurry m_sep, uncurry ( RETURN oo m)) \<in> elec_mod_sep_rel id_assn"
+  and n_sep_correct: "(uncurry n_sep, uncurry ( RETURN oo n)) \<in> elec_mod_sep_rel id_assn"
+begin
+
+                                                              
+fun sequential_composition'' :: "'a::{default, heap, hashable} Electoral_Module \<Rightarrow> 
+      'a::{default, heap, hashable} Electoral_Module \<Rightarrow>
+        'a::{default, heap, hashable} set \<Rightarrow> 'a::{default, heap, hashable} Profile 
+\<Rightarrow> 'a::{default, heap, hashable} Result nres" where
+  "sequential_composition'' ma na A pr = do {
+      (mel,mrej,mdef) <- mop_borda A pr;
+      
+      let newA = mdef;
+      new_p <- mop_limit_profile newA pr;
+    
+      (nel,nrej,ndef) <- mop_elect_module newA new_p;
+      
+      RETURN (mel \<union> nel, mrej \<union> nrej, ndef)
+}"
+
+sepref_decl_impl borda_elim_sep.refine[FCOMP borda_ref_correct, sepref_fr_rules] 
+  by simp        
+
+sepref_decl_impl elect_elect_module_sep_correct [sepref_fr_rules]
+  by simp           
+
+
+sepref_definition seqcompd is "uncurry (RETURN oo (sequential_composition'
+  elect_module borda))"
+  :: "[\<lambda>(a, b).
+           finite a ]\<^sub>a (alts_set_impl_assn id_assn)\<^sup>k *\<^sub>a 
+    (list_assn (hr_comp (ballot_impl_assn id_assn) ballot_rel))\<^sup>k 
+        \<rightarrow> (result_impl_assn id_assn)"
+  unfolding sequential_composition'.simps 
+  apply sepref_dbg_keep
+ apply sepref_dbg_trans_keep
+  oops
+  
 
 end
 
